Add fib proof

investigations/acornish/AcornEffMonad.v
@@ -32,21 +32,41 @@ Import EffMonadNotation.
 Local Open Scope eff_monad_scope.
 Local Open Scope type_scope.
 
-Class Acorn acorn `{EffMonad (list SignalType) Monoid_list_app acorn} (signal : SignalType -> Type) := {
+(* Definition state_of_type (t: SignalType) : list SignalType := *)
+(*   match t with *)
+(*   | Bit => [Bit] *)
+(*   | Nat => [Nat] *)
+(*   | Unit => [] *)
+(*   end. *)
+
+Inductive ResetValue : Type :=
+  | ResetVal : forall s, denoteSignal s -> ResetValue.
+
+Definition RNat x := ResetVal Nat x.
+Definition reset_value_type '(ResetVal s _) := s.
+Definition denote_reset '(ResetVal s _) := denoteSignal s.
+Definition reset_value_value (v: ResetValue): denote_reset v :=
+  match v as r return (denote_reset r) with
+  | ResetVal s d => d
+  end.
+
+Class Acorn acorn `{EffMonad (list ResetValue) Monoid_list_app acorn} (signal : SignalType -> Type) := {
   inv : signal Bit -> acorn [] (signal Bit);
   and2 : signal Bit * signal Bit -> acorn [] (signal Bit);
   addMod : nat -> signal Nat * signal Nat -> acorn [] (signal Nat);
-  natDelay : signal Nat -> acorn [Nat] (signal Nat);
-  loop : forall {s}, (signal Nat * signal Nat -> acorn s (signal Nat * signal Nat)) ->
-         signal Nat -> acorn (Nat::s) (signal Nat);
+  natDelay : forall rst_val, signal Nat -> acorn [RNat rst_val] (signal Nat);
+  loop : forall rst_val {i o s}, (i * signal Nat -> acorn s (o * signal Nat)) ->
+    i -> acorn (RNat rst_val::s) o;
   constNat : nat -> acorn [] (signal Nat);
   comparator : signal Nat * signal Nat -> acorn [] (signal Bit);
   mux2 : signal Bit * (signal Nat * signal Nat) -> acorn [] (signal Nat);
 }.
 
-Definition step (s: list SignalType) T := denote_list denoteSignal s -> denote_list denoteSignal s*T.
+Notation state_term x := (denote_list denote_reset x).
+Definition step (sty: list ResetValue) o :=
+  state_term sty -> state_term sty*o.
 
-Instance step_eff_monad: EffMonad (x:=list SignalType) (eff:=Monoid_list_app) step :=
+Instance step_eff_monad: EffMonad (x:=list ResetValue) (eff:=Monoid_list_app) step :=
 { ret _ x := fun _ => (tt, x)
 ; bind _ _ _ _ x f := fun s =>
   let '(sx,sf) := split_denotation _ s in
@@ -59,20 +79,26 @@ Instance AcornSimulation : Acorn step denoteSignal := {
   inv i := fun _ => (tt, negb i);
   and2 '(a, b) := fun _ => (tt, andb a b);
   addMod modBy '(a, b) := fun _ => (tt, (a + b) mod modBy);
-  natDelay i := fun '(s, tt) => (i, tt, s);
-  loop s f i := fun '(s,s_inner) =>
-    let '(ns,(o,s')) := f (i,s) s_inner in
+  natDelay rst_val i := fun '(s, tt) => (i, tt, s);
+  loop rst_val _ _ s f i := fun '(s,s_inner) =>
+    let '(ns,(o,s')) := f (i, s) s_inner in
     (s',ns,o);
   constNat n := fun _ => (tt, n);
   comparator '(a,b) := fun _ => (tt, b <=? a);
   mux2 '(sel, (a, b)) := fun _ => (tt, if sel then a else b);
 }.
 
-Definition flipper {i o s} (f: i -> s -> s * o) x y := f y x.
+Definition unpack {i o s} (f: i -> s -> s * o) x y := f y x.
+
+Fixpoint reset (st : list ResetValue): state_term st :=
+  match st with
+  | [] => tt
+  | x :: xs => (reset_value_value x, reset xs)
+  end.
 
 (* Run a circuit for many timesteps, starting at the reset value *)
-Definition simulate {i o st} (c : i -> step st o) (input : list i) : list o :=
-  fold_left_accumulate (flipper c) input (resetVals st).
+Definition simulate {i o st} (c : i -> step st o) (input : list i): list o :=
+  fold_left_accumulate (unpack c) input (reset st).
 
 Section WithAcorn.
   Context {acorn} {signal} `{Acorn acorn signal}.
@@ -101,14 +127,14 @@ Section WithAcorn.
   (* A circuit which delays the second element of a pair and then performs
      a 256-bit addition of the two values in the pair. *)
   Definition circuit1 : signal Nat * signal Nat -> acorn _ (signal Nat) :=
-    snD natDelay >=> addMod 256.
+    snD (natDelay 0) >=> addMod 256.
 
   Definition counter6 : signal Nat -> acorn _ (signal Nat) :=
     (* loop (addMod 6 >=> natDelay >=> fork2). *)
-    loop (addMod 6 >=> fork2).
+    loop 0 (addMod 6 >=> fork2).
 
   Definition nestedloop : signal Nat -> acorn _ (signal Nat) :=
-    loop (addMod 512 >=> loop (addMod 512 >=> fork2) >=> fork2).
+    loop 0 (addMod 512 >=> loop 0 (addMod 512 >=> fork2) >=> fork2).
     (* loop (snD natDelay >=> addMod 512 >=> loop (addMod 512 >=> natDelay >=> fork2) >=> fork2). *)
 
   Definition twoSorter
@@ -121,7 +147,22 @@ Section WithAcorn.
     out0 <- mux2 (comparison, (b, a)) ;;
     out1 <- mux2 (negComparison, (b, a)) ;;
     ret (out0, out1).
-  Check twoSorter.
+
+  Definition dropl {x y} (xy: signal x * signal y): acorn [] (signal y) :=
+    let '(_,y) := xy in
+    ret y.
+
+  Definition fibonacci {sz}: acorn _ (signal Nat) :=
+    loop 1 (fun '(_,r1) =>
+         r2 <- natDelay (2^sz-1) r1 ;;
+         sum <- addMod (2^sz) (r1, r2) ;;
+         fork2 sum) tt.
+
+  (* Check fibonacci. *)
+
+  (* Definition ty {x} (_:x) := x. *)
+
+  (* Eval cbv in (ty fibonacci). *)
 
 End WithAcorn.
 
@@ -167,6 +208,113 @@ Proof.
   intros. cbn in s.
   cbv [twoSorterSpec twoSorter]; cbn.
   destruct (_ <=? _); try reflexivity.
+Qed.
+
+(* Fibonacci proof *)
+
+Close Scope type_scope.
+Require Import Coq.Arith.PeanoNat.
+Require Import Coq.NArith.NArith.
+Require Import Coq.micromega.Lia.
+Require Import coqutil.Tactics.Tactics.
+Require Import Cava.Util.List.
+Require Import Cava.Util.Tactics.
+
+Fixpoint fibonacci_nat (n : nat) :=
+  match n with
+  | 0 => 0
+  | S m =>
+    let f_m := fibonacci_nat m in
+    match m with
+    | 0 => 1
+    | S p => fibonacci_nat p + f_m
+    end
+  end%nat.
+
+Definition spec_of_fibonacci (sz : nat) (input : list unit) : list nat
+  := map (fun n => fibonacci_nat n mod (2 ^ sz)) (seq 0 (List.length input)).
+
+Lemma fibonacci_step sz state :
+  fibonacci (acorn:=step) (sz:=sz) state
+  = let sum := (fst state + fst (snd state)) mod (2 ^ sz) in
+    ((sum, (fst state, tt)), sum).
+Proof.
+  intros;
+    cbv [step fibonacci];
+    cbn [fst snd natDelay addMod fork2 AcornSimulation denote_list denoteSignal loop bind].
+  repeat (destruct_pair_let;
+    cbn [fst snd bind ret step_eff_monad split_denotation combine_denotation fork2]).
+  reflexivity.
+Qed.
+
+(* jade's invariant *)
+Definition fibonacci_invariant {sz}
+           (t : nat) (loop_state : nat * (nat * unit))
+           (output_accumulator : list nat) : Prop :=
+  let r1 := fst loop_state in
+  let r2 := fst (snd loop_state) in
+  (* at timestep t... *)
+  (* ...r1 holds fibonacci_nat (t-1), or 1 if t=0 *)
+  r1 = match t with
+       | 0 => 1
+       | S t_minus1 => (fibonacci_nat t_minus1) mod (2 ^ sz)
+       end
+  (* ... and r2 holds fibonacci_nat (t-2), or 1 if t=1, 2^sz-1 if t=0 *)
+  /\ r2 = match t with
+         | 0 => 2 ^ sz - 1
+         | 1 => 1
+         | S (S t_minus2) =>(fibonacci_nat t_minus2) mod (2 ^ sz)
+         end
+  (* ... and the output accumulator matches the circuit spec for the
+     inputs so far *)
+  /\ output_accumulator = spec_of_fibonacci sz (repeat tt t).
+
+(* Helper lemma for fibonacci_correct *)
+Lemma fibonacci_nat_step n :
+  fibonacci_nat (S (S n)) = fibonacci_nat (S n) + fibonacci_nat n.
+Proof. cbn [fibonacci_nat]. lia. Qed.
+
+Lemma fibonacci_correct sz input :
+  simulate (fun _ : unit => fibonacci (sz:=sz)) input = spec_of_fibonacci sz input.
+Proof.
+  destruct input; try reflexivity.
+  cbv [simulate simulate].
+  cbn [monoid_plus Monoid_list_app resetVals resetVal app].
+
+  Set Printing Implicit.
+  rewrite fold_left_accumulate_to_seq with (default:=tt).
+  assert (2 ^ sz <> 0) by (apply Nat.pow_nonzero; lia).
+  cbv [unpack].
+  cbn [monoid_plus Monoid_list_app app ].
+  eapply fold_left_accumulate_invariant_seq with (I:=fibonacci_invariant ).
+  { cbv [fibonacci_invariant]. repeat split. }
+  { cbv [fibonacci_invariant].
+    intros. destruct_products. cbn [fst snd] in *; subst; cbn [fst snd].
+    rewrite fibonacci_step. cbn [fst snd].
+    repeat destruct_one_match.
+    { (* t = 0 case *)
+      cbn. rewrite Nat.sub_1_r, Nat.succ_pred by lia.
+      rewrite Nat.mod_same, Nat.mod_0_l by lia.
+      ssplit; reflexivity. }
+    { (* t = 1 case *)
+      cbn. rewrite Nat.mod_0_l by lia.
+      ssplit; reflexivity. }
+    { (* t > 1 case *)
+      rewrite Nat.add_mod_idemp_r, Nat.add_mod_idemp_l by lia.
+      ssplit.
+      { cbn [fibonacci_nat]. f_equal; lia. }
+      { reflexivity. }
+      { cbv [spec_of_fibonacci].
+        autorewrite with push_length.
+        rewrite seq_S with (len:=S (S _)).
+        autorewrite with natsimpl. rewrite map_app.
+        cbn [map]. rewrite fibonacci_nat_step.
+        reflexivity. } } }
+  { cbv [fibonacci_invariant]. intros.
+    logical_simplify; subst.
+    autorewrite with push_length.
+    cbn [repeat].
+    erewrite <-list_unit_equiv. reflexivity. }
 Qed.
 
 
